cleanup

src/Iris/Examples/Lithium.lean
@@ -7,6 +7,7 @@ import Iris.BI
 import Iris.ProofMode
 import Iris.Examples.IRunAttr
 import Iris.Examples.IRun
+import Iris.Examples.Exp
 
 /-
 next steps:
@@ -33,6 +34,7 @@ macro_rules
   | `($a ≫ $args) => `(.bind $a λ _ => $args)
 
 namespace HBind
+-- this does not really work
 class HBind (α : outParam (Type u)) (mα : Type v) (nβ : Type w) where
   hbind : mα → (α → nβ) → nβ
 class HPure (α : outParam (Type u)) (mα : Type v) where
@@ -51,8 +53,8 @@ structure InExM (α : Type v) where
   body : α → PROP
 
 structure LithiumM (α : Type v) where
-  body : (α → PROP) → PROP
-  mono' E1 E2 : ⊢ body E1 -∗ (∀ a, E1 a -∗ E2 a) -∗ body E2
+  run : (α → PROP) → PROP
+  mono' E1 E2 : ⊢ run E1 -∗ (∀ a, E1 a -∗ E2 a) -∗ run E2
 
 namespace InExM
 
@@ -87,7 +89,7 @@ namespace LithiumM
 variable {α : Type v} {β : Type w}
 
 def pure (a : α) : @LithiumM PROP _ α := {
-  body E := E a
+  run E := E a
   mono' E1 E2 := by
     dsimp
     iintro HE Hwand
@@ -97,16 +99,7 @@ def pure (a : α) : @LithiumM PROP _ α := {
 
 def bind (G1 : @LithiumM PROP _ α) (G2 : α → @LithiumM PROP _ β) :
   @LithiumM PROP _ β := {
-  body E := G1.body (λ a => (G2 a).body E)
-  mono' E1 E2 := by
-    dsimp
-    iintro HE Hwand
-    sorry
-}
-
-def bind2 (G1 : @LithiumM PROP _ α) (G2 : α → @LithiumM PROP _ β) :
-  @LithiumM PROP _ β := {
-  body E := G1.body (λ a => (G2 a).body E)
+  run E := G1.run (λ a => (G2 a).run E)
   mono' E1 E2 := by
     dsimp
     iintro HE Hwand
@@ -123,7 +116,7 @@ instance : HPure α (@LithiumM PROP _ α) where
   hpure := .pure
 
 def exhale (L : @InExM PROP α) : @LithiumM PROP _ α := {
-  body E := iprop(∃ a, L.body a ∗ E a)
+  run E := iprop(∃ a, L.body a ∗ E a)
   mono' E1 E2 := by
     dsimp
     iintro ⟨a, HL, HE⟩ Hwand
@@ -135,7 +128,7 @@ def exhale (L : @InExM PROP α) : @LithiumM PROP _ α := {
 }
 
 def inhale (L : @InExM PROP α) : @LithiumM PROP _ α := {
-  body E := iprop(∀ a, L.body a -∗ E a)
+  run E := iprop(∀ a, L.body a -∗ E a)
   mono' E1 E2 := by
     dsimp
     iintro HE Hwand a HL
@@ -145,7 +138,7 @@ def inhale (L : @InExM PROP α) : @LithiumM PROP _ α := {
 }
 
 def all (α : Type v) : @LithiumM PROP _ α := {
-  body E := iprop(∀ a, E a)
+  run E := iprop(∀ a, E a)
   mono' E1 E2 := by
     dsimp
     iintro HE Hwand a
@@ -155,7 +148,7 @@ def all (α : Type v) : @LithiumM PROP _ α := {
 }
 
 def done : @LithiumM PROP _ α := {
-  body E := iprop(True)
+  run E := iprop(True)
   mono' E1 E2 := by
     dsimp
     iintro HE Hwand
@@ -163,10 +156,17 @@ def done : @LithiumM PROP _ α := {
 }
 
 def lif (P : Prop) (G1 G2 : @LithiumM PROP _ α) : @LithiumM PROP _ α := {
-  body E := iprop((⌜P⌝ -∗ G1.body E) ∧ (⌜¬P⌝ -∗ G2.body E))
+  run E := iprop((⌜P⌝ -∗ G1.run E) ∧ (⌜¬P⌝ -∗ G2.run E))
   mono' E1 E2 := by
     dsimp
     iintro HE Hwand
+    sorry
+}
+
+def dsimp {α : Type _} [BI PROP] (_ : Lean.Name) (a : α) : @LithiumM PROP _ α := {
+  run E := E a
+  mono' E1 E2 := by
+    simp
     sorry
 }
 
@@ -174,7 +174,7 @@ def empty : Empty → PROP := λ e => nomatch e
 def emptyP : PEmpty → PROP := λ e => nomatch e
 
 def dualizing (G : @LithiumM PROP _ Empty) : @LithiumM PROP _ Unit := {
-  body E := iprop(G.body empty -∗ E ⟨⟩)
+  run E := iprop(G.run empty -∗ E ⟨⟩)
   mono' E1 E2 := by
     dsimp
     iintro HE Hwand HG
@@ -184,7 +184,7 @@ def dualizing (G : @LithiumM PROP _ Empty) : @LithiumM PROP _ Unit := {
 }
 
 def dualizingP (G : @LithiumM PROP _ PEmpty) : @LithiumM PROP _ PUnit := {
-  body E := iprop(G.body emptyP -∗ E ⟨⟩)
+  run E := iprop(G.run emptyP -∗ E ⟨⟩)
   mono' E1 E2 := by
     dsimp
     iintro HE Hwand HG
@@ -193,13 +193,12 @@ def dualizingP (G : @LithiumM PROP _ PEmpty) : @LithiumM PROP _ PUnit := {
     iassumption
 }
 
-def run (E : α → PROP) (G : @LithiumM PROP _ α) : PROP := G.body E
 -- TODO: What are good precedences?
-notation:35 G:36 " ⇓ " E:35 => run E G
-notation:35 G:36 " ⇓ " "!" => run empty G
+notation:35 G:36 " ⇓ " E:35 => run G E
+notation:35 G:36 " ⇓ " "!" => run G empty
 
 def entails (G1 G2 : @LithiumM PROP _ α) : Prop :=
-  ∀ E, G1.body E ⊢ G2.body E
+  ∀ E, G1.run E ⊢ G2.run E
 
 --notation:25 G1:29 ":-" G2:25 => (entails G2 G1)
 --set_option quotPrecheck false in -- TODO: Why is this necessary?
@@ -214,37 +213,37 @@ end LithiumM
 theorem run_bind (G1 : @LithiumM PROP _ α) (G2 : α → LithiumM β)
   (E : β → PROP) :
    G1.bind G2 ⇓ E ⊣ (G1 ⇓ λ b => G2 b ⇓ E) := by
-    simp [LithiumM.bind, LithiumM.body, LithiumM.run]
+    simp [LithiumM.bind, LithiumM.run, LithiumM.run]
 
 @[irun]
 theorem run_pure (a : α) (E : α → PROP) :
    .pure a ⇓ E ⊣ E a := by
-    simp [LithiumM.pure, LithiumM.body, LithiumM.run]
+    simp [LithiumM.pure, LithiumM.run, LithiumM.run]
 
 @[irun]
 theorem exhale_bind (L1 : @InExM PROP α) (L2 : α → InExM β) E :
   .exhale (L1.bind L2) ⇓ E ⊣
     LithiumM.exhale L1 ⇓ λ a => LithiumM.exhale (L2 a) ⇓ E := by
-    dsimp [bind, LithiumM.bind, LithiumM.exhale, LithiumM.body, InExM.bind, LithiumM.run]
+    dsimp [bind, LithiumM.bind, LithiumM.exhale, LithiumM.run, InExM.bind, LithiumM.run]
     sorry
 
 @[irun]
 theorem inhale_bind (L1 : @InExM PROP α) (L2 : α → InExM β) E :
   .inhale (L1.bind L2) ⇓ E ⊣
    LithiumM.inhale L1 ⇓ λ a => .inhale (L2 a) ⇓ E := by
-    dsimp [bind, LithiumM.bind, LithiumM.inhale, LithiumM.body, InExM.bind]
+    dsimp [bind, LithiumM.bind, LithiumM.inhale, LithiumM.run, InExM.bind]
     sorry
 
 @[irun]
 theorem exhale_pure (a : α) E :
   .exhale (PROP:=PROP) (.pure a) ⇓ E ⊣ E a := by
-    dsimp [bind, LithiumM.pure, LithiumM.exhale, LithiumM.body, InExM.pure]
+    dsimp [bind, LithiumM.pure, LithiumM.exhale, LithiumM.run, InExM.pure]
     sorry
 
 @[irun]
 theorem inhale_pure (a : α) E :
   .inhale (PROP:=PROP) (.pure a) ⇓ E ⊣ E a := by
-    dsimp [bind, LithiumM.pure, LithiumM.inhale, LithiumM.body, InExM.pure]
+    dsimp [bind, LithiumM.pure, LithiumM.inhale, LithiumM.run, InExM.pure]
     sorry
 
 
@@ -319,7 +318,7 @@ theorem inhale_own_tac [BI PROP] {P A : PROP} (E : Unit → PROP)
 def irunInhaleOwn : IRunTacticType := fun goal => do profileitM Exception "irunIntro" (← getOptions) do
   let g ← instantiateMVars <| ← goal.getType
   let some { prop, bi, e, hyps, goal:=G } := parseIrisGoal? g | throwError "not in proof mode"
-  let ~q(LithiumM.run $E (LithiumM.inhale (.own $A))) := G | return none
+  let ~q(LithiumM.run (LithiumM.inhale (.own $A)) $E) := G | return none
   let ident ← `(binderIdent| _)
   let (b, A') := if A.isAppOfArity ``intuitionistically 3 then
       (q(true), A.getArg! 3)
@@ -341,7 +340,6 @@ theorem cancel [BI PROP] {p : Bool} {P P' A : PROP} {E}
   (h : P' ⊢ E ())
  : P ⊢ LithiumM.exhale (.own A) ⇓ E := by
    sorry
-   --hP.1.trans <| sep_comm.1.trans <| sep_mono intuitionisticallyIf_elim h
 
 @[irun_tac LithiumM.exhale (InExM.own _) ⇓ _]
 def irunCancel : IRunTacticType := fun goal => do profileitM Exception "irunCancel" (← getOptions) do
@@ -371,7 +369,7 @@ def irunDone : IRunTacticType := fun goal => do profileitM Exception "irunTrue" 
   let g ← instantiateMVars <| ← goal.getType
   let some { prop:=prop, bi:=bi, hyps:=_, e, goal:=G } := parseIrisGoal? g | throwError "not in proof mode"
   match_expr G with
-  | LithiumM.run _ _ α E G =>
+  | LithiumM.run _ _ α G E =>
     let .true := G.isAppOfArity ``LithiumM.done 3 | return none
     let pf := mkApp5 (.const ``done_tac G.getAppFn.constLevels!) prop α bi e E
     goal.assign pf
@@ -392,10 +390,10 @@ theorem lif_false {α : Type _} [BI PROP] {cond} {P : PROP} (G1 : LithiumM α) G
    sorry
 
 syntax "istepsolve" : tactic
---macro_rules
---  | `(tactic|istepsolve) => `(tactic|trivial)
 macro_rules
-  | `(tactic|istepsolve) => `(tactic|solve| simp)
+  | `(tactic|istepsolve) => `(tactic|trivial)
+--macro_rules
+--  | `(tactic|istepsolve) => `(tactic|solve| simp)
 
 @[irun_tac LithiumM.lif _ _ _ ⇓ _]
 def irunLif : IRunTacticType := fun goal => do profileitM Exception "irunLif" (← getOptions) do
@@ -425,6 +423,20 @@ def irunLif : IRunTacticType := fun goal => do profileitM Exception "irunLif" (�
 
   throwError "Cannot solve either side of lif"
 
+@[irun_tac LithiumM.dsimp _ _ ⇓ _]
+def irunSimp : IRunTacticType := fun goal => do profileitM Exception "irunSimp" (← getOptions) do
+  let g ← instantiateMVars <| ← goal.getType
+  let some ig := parseIrisGoal? g | throwError "not in proof mode"
+  let { prop:=_, bi:=_, e:=_, hyps:=_, goal:=G } := ig
+
+  let_expr LithiumM.run _ _ _ G E := G | return none
+  let_expr LithiumM.dsimp _ _ _ n e := G | return none
+  let n : Name ← reduceEval n
+  let ⟨e_new, _⟩ ← goal.withContext (dsimpWithExt n e)
+  let g' := {ig with goal := Expr.beta E #[e_new]}.toExpr
+  let goal' := ← goal.replaceTargetDefEq g'
+  return .some ([goal'], [])
+
 section test
 variable {u} [BI.{u} PROP]
 
@@ -451,7 +463,7 @@ theorem test_intro_cancel (P G : PROP) :
     irun 1
     irun 1
 
-/-
+
 --set_option profiler true in
 --set_option profiler.threshold 1 in
 set_option maxRecDepth 30000 in
@@ -479,8 +491,8 @@ set_option maxRecDepth 30000 in
       (.done ⇓ !) (
     -- List.reverse makes cancellation basically instant
     -- List.reverse
-    (List.range 100)))
-    (List.range 100))
+    (List.range 2)))
+    (List.range 2))
 :=
   by
     dsimp [List.foldl, List.range, List.range.loop, List.reverse]
@@ -489,46 +501,15 @@ set_option maxRecDepth 30000 in
     -- set_option trace.profiler.threshold 1 in
     -- irun ∞
     sorry
--/
 
 end test
 
 end Iris.ProofMode
 
 namespace Iris.Examples
-open Lithium
+open Lang Lithium
 
-section lang
 variable {u} [BI.{u} PROP]
-def Loc : Type := Nat
-
-inductive Binop where
-| plus | minus | eq
-
-mutual
-inductive Val where
-| nat : Nat -> Val
-| loc : Loc -> Val
-| recv : String -> String -> Exp -> Val
-inductive Exp where
-| val : Val -> Exp
-| var : String -> Exp
-| binop : Exp -> Binop -> Exp -> Exp
-| rece : String -> String -> Exp -> Exp
-| app : Exp -> Exp -> Exp
-| ife : Exp -> Exp -> Exp -> Exp
-end
-
-def subst (x : String) (v : Val) (e : Exp) : Exp :=
-  match e with
-  | .val _ => e
-  | .var y => if x == y then .val v else e
-  | .binop e1 o e2 => .binop (subst x v e1) o (subst x v e2)
-  | .rece f y e' => .rece f y (if x == f || x == y then e' else subst x v e')
-  | .app e1 e2 => .app (subst x v e1) (subst x v e2)
-  | .ife e1 e2 e3 => .ife (subst x v e1) (subst x v e2)  (subst x v e3)
-
-def wp [BI PROP] (e : Exp) (P : Val -> PROP) : PROP := by sorry
 
 theorem wp_wand e (P1 P2 : Val -> PROP) :
   ⊢ wp e P1 -∗ (∀ v, P1 v -∗ P2 v) -∗ wp e P2
@@ -538,23 +519,23 @@ theorem wp_wand e (P1 P2 : Val -> PROP) :
 /- Proof automation begins here -/
 
 def expr_ok (e : Exp) : @LithiumM PROP _ Val := {
-  body := wp e
+  run := wp e
   mono' := wp_wand e
 }
 
 def expr_okP (e : Exp) : @LithiumM PROP _ (ULift.{u} Val) := {
-  body E := wp e (λ v => E (ULift.up v))
+  run E := wp e (λ v => E (ULift.up v))
   mono' := by sorry
 }
 
 /- problem: Monad is not fully universe polymorphic -/
 def fn_specP (v : Val) (G : Val → @LithiumM PROP _ (Val → @LithiumM PROP _ PEmpty)) : PROP :=
   iprop(∀ (E : ULift.{u} Val → PROP) va,
-  (LithiumM.run E do
+  (do
     let L' : Val → LithiumM PEmpty ← G va
     let vr ← .all (ULift.{u} Val)
     LithiumM.dualizingP (L' vr.down)
-    return vr)
+    return vr) ⇓ E
   -∗
   wp (.app (.val v) (.val va)) λ v => E (ULift.up v))
 
@@ -570,17 +551,17 @@ def fn_spec (v : Val) (G : Val → @LithiumM PROP _ (Val → @LithiumM PROP _ Em
   wp (.app (.val v) (.val va)) E)
 
 def nat_ok (v : Val) : @LithiumM PROP _ Nat := {
-  body E := iprop(∃ n, ⌜v = .nat n⌝ ∗ E n)
+  run E := iprop(∃ n, ⌜v = .nat n⌝ ∗ E n)
   mono' E1 E2 := by sorry
 }
 
 def recv_ok (v : Val) : @LithiumM PROP _ (String × String × Exp) := {
-  body E := iprop(∃ f x e, ⌜v = .recv f x e⌝ ∗ E (f, x, e))
+  run E := iprop(∃ f x e, ⌜v = .recv f x e⌝ ∗ E (f, x, e))
   mono' E1 E2 := by sorry
 }
 
 def subst_ok (x : String) (v : Val) (e : Exp) : @LithiumM PROP _ Exp := {
-  body E := E (subst x v e)
+  run E := E (subst x v e)
   mono' E1 E2 := by
     simp
     sorry
@@ -589,7 +570,7 @@ def subst_ok (x : String) (v : Val) (e : Exp) : @LithiumM PROP _ Exp := {
 @[irun]
 theorem nat_ok_nat (n : Nat) (E : Nat → PROP) :
   nat_ok (.nat n) ⇓ E ⊣ E n := by
-  dsimp [nat_ok, LithiumM.run, LithiumM.body]
+  dsimp [nat_ok, LithiumM.run, LithiumM.run]
   iintro HP
   iexists _
   isplit
@@ -600,7 +581,7 @@ theorem nat_ok_nat (n : Nat) (E : Nat → PROP) :
 @[irun]
 theorem recv_ok_rec f x e (E : (String × String × Exp) -> PROP) :
   recv_ok (.recv f x e) ⇓ E ⊣ E (f, x, e) := by
-  dsimp [recv_ok, LithiumM.run, LithiumM.body]
+  dsimp [recv_ok, LithiumM.run, LithiumM.run]
   iintro HP
   iexists _
   iexists _
@@ -620,7 +601,9 @@ theorem expr_ok_plus e1 e2 (E : Val -> PROP) :
    expr_ok e1 ⇓ λ v1 =>
    expr_ok e2 ⇓ λ v2 =>
    nat_ok v1 ⇓ λ n1 =>
-   nat_ok v2 ⇓ λ n2 => E (.nat (n1 + n2)) := by sorry
+   nat_ok v2 ⇓ λ n2 =>
+   .dsimp `irun_simp (n1 + n2) ⇓ λ n =>
+   E (.nat n) := by sorry
 
 @[irun]
 theorem expr_ok_minus e1 e2 (E : Val -> PROP) :
@@ -628,7 +611,9 @@ theorem expr_ok_minus e1 e2 (E : Val -> PROP) :
    expr_ok e1 ⇓ λ v1 =>
    expr_ok e2 ⇓ λ v2 =>
    nat_ok v1 ⇓ λ n1 =>
-   nat_ok v2 ⇓ λ n2 => E (.nat (n1 - n2)) := by sorry
+   nat_ok v2 ⇓ λ n2 =>
+   .dsimp `irun_simp (n1 - n2) ⇓ λ n =>
+   E (.nat n) := by sorry
 
 @[irun]
 theorem expr_ok_eq e1 e2 (E : Val -> PROP) :
@@ -636,7 +621,9 @@ theorem expr_ok_eq e1 e2 (E : Val -> PROP) :
    expr_ok e1 ⇓ λ v1 =>
    expr_ok e2 ⇓ λ v2 =>
    nat_ok v1 ⇓ λ n1 =>
-   nat_ok v2 ⇓ λ n2 => E (.nat (if n1 == n2 then 1 else 0)) := by sorry
+   nat_ok v2 ⇓ λ n2 =>
+   .dsimp `irun_simp (if n1 == n2 then 1 else 0) ⇓ λ n =>
+   E (.nat n) := by sorry
 
 @[irun]
 theorem expr_ok_rec f x e (E : Val -> PROP) :
@@ -659,64 +646,10 @@ theorem expr_ok_if e1 e2 e3 (E : Val -> PROP) :
    LithiumM.lif (n1 ≠ 0) (expr_ok e2) (expr_ok e3) ⇓ E) ⊢
   expr_ok (.ife e1 e2 e3) ⇓ E := by sorry
 
-namespace Reify
-open Lean
-inductive Exp where
-| val : Expr -> Exp -- we do not need to reify values
-| var : String -> Exp
-| binop : Exp -> Expr -> Exp -> Exp
-| rece : String -> String -> Exp -> Exp
-| app : Exp -> Exp -> Exp
-| ife : Exp -> Exp -> Exp -> Exp
-| unk : Expr -> Exp
-deriving Inhabited, Repr
-
--- should this be ToExpr?
-def Exp.unreify : Exp → Expr
-  | .val v => mkApp (mkConst ``Examples.Exp.val) v
-  | .var v => mkApp (mkConst ``Examples.Exp.var) (mkStrLit v)
-  | .binop e1 o e2 => mkApp3 (mkConst ``Examples.Exp.binop) (unreify e1) o (unreify e2)
-  | .rece f x e => mkApp3 (mkConst ``Examples.Exp.rece) (mkStrLit f) (mkStrLit x) (unreify e)
-  | .app e1 e2 => mkApp2 (mkConst ``Examples.Exp.app) (unreify e1) (unreify e2)
-  | .ife e1 e2 e3 => mkApp3 (mkConst ``Examples.Exp.ife) (unreify e1) (unreify e2) (unreify e3)
-  | .unk e => e
-
-
-def rawStringLit? : Expr → Option String
-  | .lit (.strVal v) => .some v
-  | _ => .none
-
-
-partial def reify (e : Expr) : Exp :=
-  match_expr e with
-  | Examples.Exp.val v => .val v
-  | Examples.Exp.var v =>
-    match v with
-    | .lit (.strVal v) => .var v
-    | _ => .unk e
-  | Examples.Exp.binop e1 o e2 => .binop (reify e1) o (reify e2)
-  | Examples.Exp.rece f x e' =>
-    match f, x with
-    | .lit (.strVal f), .lit (.strVal x) => .rece f x (reify e')
-    | _, _ => .unk e'
-  | Examples.Exp.app e1 e2 => .app (reify e1) (reify e2)
-  | Examples.Exp.ife e1 e2 e3 => .ife (reify e1) (reify e2) (reify e3)
-  | _ => .unk e
-
-def subst (x : String) (v : Expr) (e : Exp) : Exp :=
-  match e with
-  | .val _ => e
-  | .var y => if x = y then .val v else e
-  | .binop e1 o e2 => .binop (subst x v e1) o (subst x v e2)
-  | .rece f y e' => .rece f y (if x == f || x == y then e' else subst x v e')
-  | .app e1 e2 => .app (subst x v e1) (subst x v e2)
-  | .ife e1 e2 e3 => .ife (subst x v e1) (subst x v e2)  (subst x v e3)
-  | .unk e => .unk (mkApp3 (mkConst ``Examples.subst) (mkStrLit x) v e)
-
-end Reify
 
 section
 open Lean Elab Tactic Meta Qq BI Std ProofMode
+
 @[irun_tac subst_ok _ _ _ ⇓  _]
 def irunSubst : IRunTacticType := fun goal => do profileitM Exception "irunSubst" (← getOptions) do
   let g ← instantiateMVars <| ← goal.getType
@@ -724,32 +657,19 @@ def irunSubst : IRunTacticType := fun goal => do profileitM Exception "irunSubst
   let { prop:=_, bi:=_, e:=_, hyps:=_, goal:=G } := ig
 
   let .true := G.isAppOfArity ``LithiumM.run 5 | return none
-  let E := G.getArg! 3
-  let G' := G.getArg! 4
+  let G' := G.getArg! 3
+  let E := G.getArg! 4
   let .true := G'.isAppOfArity ``subst_ok 5 | return none
-  let .some x := Reify.rawStringLit? (G'.getArg! 2) | return none
+  let .lit (.strVal x) := G'.getArg! 2 | return none
   let v := G'.getArg! 3
   let e := Reify.reify (G'.getArg! 4)
   let e' := (Reify.subst x v e).unreify
---  let e' ← whnfR (mkApp3 (mkConst ``subst) (G'.getArg! 2) (G'.getArg! 3) (G'.getArg! 4))
---  logInfo m!"{repr e}"
---  logInfo m!"{e'}"
-  -- TODO: Do something smarter here?
   let g' := {ig with goal := Expr.beta E #[e']}.toExpr
-  let { ctx:=simpctx, simprocs, .. } ← mkSimpContext .missing (eraseLocal := false) (kind := .dsimp)
-  let ⟨g', _⟩ ← Meta.dsimp g' simpctx simprocs
+--  let ⟨g', _⟩ ← goal.withContext (dsimpWithExt `irun_simp g')
   let goal' := ← goal.replaceTargetDefEq g'
-  -- let goals ← evalTacticAtRaw (← `(tactic | (conv => rhs; arg 0; unfold LithiumM.run) <;> (conv => rhs; arg 1; unfold subst_ok) <;> dsimp [LithiumM.body, subst])) goal
---  let goals ← evalTacticAtRaw (← `(tactic | dsimp [LithiumM.run, subst_ok, subst])) goal
-  -- let goals ← evalTacticAtRaw (← `(tactic | try dsimp)) goal'
   return .some ([goal'], [])
-  -- return .some (goals, [])
 
 end
-end lang
-
-section
-variable {u} [BI.{u} PROP]
 
 theorem expr_ok_test (P : Val -> PROP) :
   ⊢ .inhale (.own (P (.nat 10))) ⇓ λ _ =>
@@ -765,9 +685,8 @@ theorem expr_ok_test (P : Val -> PROP) :
   irun 1
   irun 1
   irun 1
+  irun 1
 
-def rec_fn : Val :=
-  .recv "f" "x" (.ife (.binop (.var "x") .eq (.val (.nat 0))) (.val (.nat 0)) (.app (.var "f") (.binop (.var "x") .minus (.val (.nat 1)))))
 
 attribute [irun_simp] Nat.add_one_sub_one
 
@@ -780,12 +699,10 @@ set_option profiler true in
       .done ⇓ ! := by
   istart
   unfold rec_fn
-  --isubst <;> iautoapply
   --set_option trace.profiler true in
   --set_option trace.profiler.threshold 1 in
   --set_option diagnostics true in
   --set_option profiler true in
   irun ∞
 
-end
 end Iris.Examples
