src/Iris/Examples/Exp.lean
@@ -1,0 +1,94 @@
+/-
+Copyright (c) 2025 Michael Sammler. All rights reserved.
+Released under Apache 2.0 license as described in the file LICENSE.
+Authors: Michael Sammler
+-/
+import Iris.BI
+import Iris.ProofMode
+
+namespace Iris.Examples.Lang
+open BI
+
+variable {u} [BI.{u} PROP]
+
+def Loc : Type := Nat
+
+inductive Binop where
+| plus | minus | eq
+
+mutual
+inductive Val where
+| nat : Nat -> Val
+| loc : Loc -> Val
+| recv : String -> String -> Exp -> Val
+inductive Exp where
+| val : Val -> Exp
+| var : String -> Exp
+| binop : Exp -> Binop -> Exp -> Exp
+| rece : String -> String -> Exp -> Exp
+| app : Exp -> Exp -> Exp
+| ife : Exp -> Exp -> Exp -> Exp
+end
+
+def subst (x : String) (v : Val) : Exp → Exp
+  | .val v => .val v
+  | .var y => if x == y then .val v else .var y
+  | .binop e1 o e2 => .binop (subst x v e1) o (subst x v e2)
+  | .rece f y e' => .rece f y (if x == f || x == y then e' else subst x v e')
+  | .app e1 e2 => .app (subst x v e1) (subst x v e2)
+  | .ife e1 e2 e3 => .ife (subst x v e1) (subst x v e2)  (subst x v e3)
+
+def wp [BI PROP] (e : Exp) (P : Val -> PROP) : PROP := by sorry
+
+namespace Reify
+open Lean
+inductive Exp where
+| val : Expr -> Exp -- we do not need to reify values
+| var : String -> Exp
+| binop : Exp -> Expr -> Exp -> Exp
+| rece : String -> String -> Exp -> Exp
+| app : Exp -> Exp -> Exp
+| ife : Exp -> Exp -> Exp -> Exp
+| unk : Expr -> Exp
+deriving Inhabited, Repr
+
+-- should this be ToExpr?
+def Exp.unreify : Exp → Expr
+  | .val v => mkApp (mkConst ``Lang.Exp.val) v
+  | .var v => mkApp (mkConst ``Lang.Exp.var) (mkStrLit v)
+  | .binop e1 o e2 => mkApp3 (mkConst ``Lang.Exp.binop) (unreify e1) o (unreify e2)
+  | .rece f x e => mkApp3 (mkConst ``Lang.Exp.rece) (mkStrLit f) (mkStrLit x) (unreify e)
+  | .app e1 e2 => mkApp2 (mkConst ``Lang.Exp.app) (unreify e1) (unreify e2)
+  | .ife e1 e2 e3 => mkApp3 (mkConst ``Lang.Exp.ife) (unreify e1) (unreify e2) (unreify e3)
+  | .unk e => e
+
+partial def reify (e : Expr) : Exp :=
+  match_expr e with
+  | Lang.Exp.val v => .val v
+  | Lang.Exp.var v =>
+    match v with
+    | .lit (.strVal v) => .var v
+    | _ => .unk e
+  | Lang.Exp.binop e1 o e2 => .binop (reify e1) o (reify e2)
+  | Lang.Exp.rece f x e' =>
+    match f, x with
+    | .lit (.strVal f), .lit (.strVal x) => .rece f x (reify e')
+    | _, _ => .unk e'
+  | Lang.Exp.app e1 e2 => .app (reify e1) (reify e2)
+  | Lang.Exp.ife e1 e2 e3 => .ife (reify e1) (reify e2) (reify e3)
+  | _ => .unk e
+
+def subst (x : String) (v : Expr) (e : Exp) : Exp :=
+  match e with
+  | .val _ => e
+  | .var y => if x == y then .val v else e
+  | .binop e1 o e2 => .binop (subst x v e1) o (subst x v e2)
+  | .rece f y e' => .rece f y (if x == f || x == y then e' else subst x v e')
+  | .app e1 e2 => .app (subst x v e1) (subst x v e2)
+  | .ife e1 e2 e3 => .ife (subst x v e1) (subst x v e2)  (subst x v e3)
+  | .unk e => .unk (mkApp3 (mkConst ``Lang.subst) (mkStrLit x) v e)
+
+end Reify
+
+def rec_fn : Val :=
+  .recv "f" "x" (.ife (.binop (.var "x") .eq (.val (.nat 0))) (.val (.nat 0)) (.app (.var "f") (.binop (.var "x") .minus (.val (.nat 1)))))
